kosaraju-tarjan-lean4/Graph/DirectedGraph.lean
@@ -1,12 +1,12 @@
-import Std.Data.List.Basic
-import Std.Data.List.Lemmas
+import Init.Data.List.Basic
+import Init.Data.List.Lemmas
 import Mathlib.Data.Finset.Basic
 import Mathlib.Tactic.Use
 import Mathlib.Tactic.Tauto
 import ListHelper.Simplelist
 
 -- finite directed graph
-class DirectedGraph (V : Type u)(Graph : Type v) where
+class DirectedGraph (V : Type*)(Graph : Type*) where
   vertices : Graph -> List V
   succ      : Graph -> V -> List V
   edge      : Graph -> V -> V -> Prop := fun g x y => y ∈ succ g x
@@ -17,7 +17,7 @@ class DirectedGraph (V : Type u)(Graph : Type v) where
   same_vertices : ∀ g, (g |> transpose |> vertices) = (g |> vertices)
   reverse_edge :∀ g a b, edge g a b <-> edge (g |> transpose) b a
 
-theorem succ_valid [DirectedGraph V Graph] (g : Graph) (a: V)
+theorem succ_valid {V Graph : Type*} [DirectedGraph V Graph] (g : Graph) (a: V)
   (_ : a ∈ DirectedGraph.vertices g) :
   DirectedGraph.succ g a ⊆ DirectedGraph.vertices g := by
 intro b h
@@ -27,18 +27,18 @@ have : a ∈ DirectedGraph.vertices g /\ b ∈ DirectedGraph.vertices g := by
   assumption
 tauto
 
-inductive path [DirectedGraph V Graph] : Graph -> V -> List V -> V -> Prop
+inductive path {V Graph : Type*} [DirectedGraph V Graph] : Graph -> V -> List V -> V -> Prop
   | edge: ∀ (g: Graph) (a b: V), DirectedGraph.edge g a b -> path g a List.nil b
   | cons: ∀ (g: Graph) (a b c: V) (l: List V), DirectedGraph.edge g a b -> path g b l c -> path g a (List.cons b l) c
 
-theorem path_trans [DirectedGraph V Graph] (g : Graph) (a b c: V) (lab lbc: List V)
+theorem path_trans {V Graph : Type*} [DirectedGraph V Graph] (g : Graph) (a b c: V) (lab lbc: List V)
         (h : path g a lab b) :
         path g b lbc c -> path g a (lab ++ List.cons b lbc) c := by
 induction h
 . simp; intros; constructor <;> assumption
 . intros; simp_all; constructor <;> assumption
 
-theorem path_decomposition [DirectedGraph V Graph] (g : Graph) (a b c: V) (lab lbc: List V) :
+theorem path_decomposition {V Graph : Type*} [DirectedGraph V Graph] (g : Graph) (a b c: V) (lab lbc: List V) :
   path g a (lab ++ List.cons b lbc) c -> path g a lab b /\ path g b lbc c := by
 revert a b c lbc
 induction lab <;> simp_all <;> intros a b c lbc h <;> cases h
@@ -47,7 +47,7 @@ induction lab <;> simp_all <;> intros a b c lbc h <;> cases h
   specialize induction_step x b c lbc h₃
   tauto
 
-theorem reverse_path [DirectedGraph V Graph] (g : Graph) (a b : V) (l : List V)
+theorem reverse_path {V Graph : Type*} [DirectedGraph V Graph] (g : Graph) (a b : V) (l : List V)
         (h : path g a l b) : path (DirectedGraph.transpose V g) b l.reverse a := by
 induction h <;> simp
 . constructor; rw [<- DirectedGraph.reverse_edge]; assumption
@@ -55,7 +55,7 @@ induction h <;> simp
   . assumption
   . constructor; rw [<- DirectedGraph.reverse_edge]; assumption
 
-theorem path_valid [DirectedGraph V Graph] (g : Graph) (a b: V)(l : List V)
+theorem path_valid {V Graph : Type*} [DirectedGraph V Graph] (g : Graph) (a b: V)(l : List V)
         (h : path g a l b) :
         a ∈ DirectedGraph.vertices g /\
         b ∈ DirectedGraph.vertices g /\
@@ -70,7 +70,8 @@ induction h <;> simp_all
     assumption
   tauto
 
-def reachable [DirectedGraph V Graph]
+def reachable {V Graph : Type*}
+              [DirectedGraph V Graph]
               [BEq V] [LawfulBEq V]
               (g : Graph)
               (a b : V)
@@ -81,7 +82,8 @@ def reachable [DirectedGraph V Graph]
                             a = b /\ a ∈ v
                           )
 
-theorem reachable_trans [DirectedGraph V Graph]
+theorem reachable_trans {V Graph : Type*}
+                        [DirectedGraph V Graph]
                         [BEq V] [LawfulBEq V]
                         (g : Graph)
                         (x y z : V) :
@@ -100,7 +102,8 @@ all_goals rename_i h g
   subst z
   assumption
 
-theorem reachable_valid [DirectedGraph V Graph]
+theorem reachable_valid {V Graph : Type*}
+                        [DirectedGraph V Graph]
                         [BEq V] [LawfulBEq V]
                         (g : Graph) (a b: V)
                         (h : reachable g a b) :
@@ -115,56 +118,64 @@ cases h with
            tauto
 
 
-def no_black_to_white [DirectedGraph V Graph]
+def no_black_to_white {V Graph Lv: Type*}
+                      [DirectedGraph V Graph]
                       [BEq V] [LawfulBEq V]
                       [Membership V Lv]
                       (g : Graph)
                       (blacks grays: Lv) : Prop :=
     ∀ a b, DirectedGraph.edge g a b -> a ∈ blacks -> b ∈ grays \/ b ∈ blacks
 
-def access_from_set [DirectedGraph V Graph]
+def access_from_set {V Graph : Type*}
+                    [DirectedGraph V Graph]
                     [BEq V] [LawfulBEq V]
                     (g : Graph)
                     (roots b: List V) : Prop :=
 ∀ z ∈ b, ∃ x ∈ roots, reachable g x z
 
-def access_to [DirectedGraph V Graph]
+def access_to {V Graph : Type*}
+              [DirectedGraph V Graph]
               [BEq V] [LawfulBEq V]
               (graph : Graph)(s: Finset V) (y: V) : Prop :=
 ∀ x ∈ s, reachable graph x y
 
-def wff_color [DirectedGraph V Graph]
+def wff_color {V Graph : Type*}
+              [DirectedGraph V Graph]
               [BEq V] [LawfulBEq V]
               (g : Graph)
               (blacks grays: List V) : Prop :=
               (∀ x, x ∈ blacks -> x ∈ grays -> False) /\
               no_black_to_white g blacks grays /\
-              simplelist blacks /\
-              simplelist grays
+              List.Nodup blacks /\
+              List.Nodup grays
 
 
-def no_edge_out_of [DirectedGraph V Graph]
+def no_edge_out_of {V Graph : Type*}
+                   [DirectedGraph V Graph]
                    [BEq V] [LawfulBEq V]
                    (g : Graph)
                    (s3 s1: List V) : Prop :=
     ∀ s2, s1 = s2 ++ s3 -> ∀ x y, x ∈ s3 -> y ∈ s2 -> DirectedGraph.edge g x y -> False
 
-def no_path_out_of_in [DirectedGraph V Graph]
+def no_path_out_of_in {V Graph : Type*}
+                      [DirectedGraph V Graph]
                       [BEq V] [LawfulBEq V]
                       (g : Graph)
                       (s3 s1: List V) : Prop :=
     ∀ x y l s2, s1 = s2 ++ s3 -> x ∈ s3 -> y ∈ s2 -> path g x l y -> l ⊆ s1 -> False
 
-def paths_in_set [DirectedGraph V Graph]
+def paths_in_set {V Graph : Type*}
+                 [DirectedGraph V Graph]
                  [BEq V] [LawfulBEq V]
                  (g : Graph)
                  (cc: List V) : Prop :=
     ∀ x l y, x ∈ cc -> y ∈ cc -> path g x l y -> l ⊆ cc
 
-theorem reachable_transpose [DirectedGraph V Graph]
-                              [BEq V] [LawfulBEq V]
-                              (g : Graph)
-                              (a b : V) :
+theorem reachable_transpose {V Graph : Type*}
+                            [DirectedGraph V Graph]
+                            [BEq V] [LawfulBEq V]
+                            (g : Graph)
+                            (a b : V) :
 reachable (DirectedGraph.transpose V g) a b <-> reachable g b a := by
 simp [reachable]
 rw [DirectedGraph.same_vertices]
