kosaraju-tarjan-lean4/Graph/ReachableBefore.lean
@@ -2,7 +2,8 @@ import Graph.DirectedGraph
 import Graph.Scc
 import ListHelper.Rank
 
-def reachable_before [DirectedGraph V Graph]
+def reachable_before {V Graph: Type*}
+                     [DirectedGraph V Graph]
                      [BEq V] [LawfulBEq V]
                      (g : Graph)
                      (x y: V) (s: List V) : Prop :=
@@ -15,14 +16,16 @@ def reachable_before [DirectedGraph V Graph]
   \/
   (x = y /\ x ∈ s)
 
-def reachable_before_same_scc [DirectedGraph V Graph]
+def reachable_before_same_scc {V Graph: Type*}
+                              [DirectedGraph V Graph]
                               [BEq V] [LawfulBEq V]
                               (g : Graph)
                               (s: List V) : Prop :=
    ∀ x y, x ∈ s -> y ∈ s -> reachable_before g x y s -> in_same_scc g x y
 
 
-def wff_stack_G1 [DirectedGraph V Graph]
+def wff_stack_G1 {V Graph: Type*}
+                 [DirectedGraph V Graph]
                  [BEq V] [LawfulBEq V]
                  (g : Graph)
                  (blacks grays: List V) :=
@@ -30,16 +33,18 @@ def wff_stack_G1 [DirectedGraph V Graph]
     /\ blacks ⊆ (DirectedGraph.vertices g)
     /\ reachable_before_same_scc g blacks
 
-def wff_stack_G2 [DirectedGraph V Graph]
+def wff_stack_G2 {V Graph: Type*}
+                 [DirectedGraph V Graph]
                  [BEq V] [LawfulBEq V]
                  (g : Graph)
                  (blacks grays s: List V) :=
     wff_color g blacks grays
-    /\ simplelist s
+    /\ List.Nodup s
     /\ s ⊆ DirectedGraph.vertices g
     /\ reachable_before_same_scc (DirectedGraph.transpose V g) s
 
-theorem reachable_before_shrink [DirectedGraph V Graph]
+theorem reachable_before_shrink {V Graph: Type*}
+                                [DirectedGraph V Graph]
                                 [BEq V] [LawfulBEq V]
                                 (g : Graph) :
 ∀ (x y z: V) s, reachable_before g x y (List.cons z s) -> y ∈ s -> reachable_before g x y s := by
@@ -86,7 +91,8 @@ theorem reachable_before_shrink [DirectedGraph V Graph]
               tauto
 
 
-theorem reachable_before_extension [DirectedGraph V Graph]
+theorem reachable_before_extension {V Graph: Type*}
+                                   [DirectedGraph V Graph]
                                    [BEq V] [LawfulBEq V]
                                    (g : Graph) :
   ∀ (x y z: V) s, x ∈ s -> y ∈ s -> reachable_before g x y s -> reachable_before g x y (List.cons z s) := by
@@ -114,7 +120,8 @@ theorem reachable_before_extension [DirectedGraph V Graph]
               subst y
               tauto
 
-theorem no_edge_out_of_cons [DirectedGraph V Graph]
+theorem no_edge_out_of_cons {V Graph: Type*}
+                            [DirectedGraph V Graph]
                             [BEq V] [LawfulBEq V]
                             (g : Graph)
                             (s1 s2: List V) (x : V) :
@@ -129,11 +136,12 @@ theorem no_edge_out_of_cons [DirectedGraph V Graph]
                     specialize h₁ a b h₄
                     cases h₅ <;> simp_all
 
-theorem path_cross_sets [DirectedGraph V Graph]
+theorem path_cross_sets {V Graph: Type*}
+                        [DirectedGraph V Graph]
                         [BEq V] [LawfulBEq V]
                         (g : Graph) :
    ∀ l (x y : V) s1 s2 ,
-   -- simplelist (s1 ++ s2) ->
+   -- List.Nodup (s1 ++ s2) ->
    y ∈ s2 ->
    x ∈ s1 ->
    path g y l x ->
@@ -156,11 +164,12 @@ theorem path_cross_sets [DirectedGraph V Graph]
          apply h₄
          simp_all
 
-theorem no_edge_out_of_no_path_out_of_in [DirectedGraph V Graph]
+theorem no_edge_out_of_no_path_out_of_in {V Graph: Type*}
+                                        [DirectedGraph V Graph]
                                         [BEq V] [LawfulBEq V]
                                         (g : Graph) :
     ∀ (s1 s2 : List V),
-   --  simplelist s2 ->
+   --  List.Nodup s2 ->
     no_edge_out_of g s1 s2 -> no_path_out_of_in g s1 s2 := by
 simp [no_edge_out_of, no_path_out_of_in]
 intros s2 s3 h₁ x y l s1 h₂ h₃ h₄ h₅ h₆
@@ -172,7 +181,8 @@ obtain ⟨x, y, h₂, h₃, h₄⟩ := h₇
 apply h₁ x y h₂ h₃ h₄
 
 
-theorem no_black_to_white_no_path [DirectedGraph V Graph]
+theorem no_black_to_white_no_path {V Graph: Type*}
+                                [DirectedGraph V Graph]
                                 [BEq V] [LawfulBEq V]
                                 (g : Graph) :
 ∀ (b : List V),
@@ -186,7 +196,8 @@ induction l <;> intros x y h₂ h₃ h₄ <;> cases h₄
   have h₆ : z ∈ b \/ ¬ z ∈ b := by tauto
   cases h₆ <;> tauto
 
-theorem no_black_to_white_in_the_middle [DirectedGraph V Graph]
+theorem no_black_to_white_in_the_middle {V Graph: Type*}
+                                        [DirectedGraph V Graph]
                                         [BEq V] [LawfulBEq V]
                                         (g : Graph) :
 ∀ (b b' : List V), no_black_to_white g b  List.nil ->
@@ -194,20 +205,16 @@ theorem no_black_to_white_in_the_middle [DirectedGraph V Graph]
                       b ⊆ b' ->
                       paths_in_set g (List.filter (fun x => !b.contains x) b') := by
 simp [paths_in_set]
-intros b b' h₁ h₂ _ x l y h₄ h₅ h₆ z h₇
+intros b b' h₁ h₂ _ x l y h₄ h₅ h₆ z h₇ z hz
 rw [List.mem_filter] at *
 simp_all
-have h₈ := List.append_of_mem h₇
+have h₈ := List.append_of_mem hz
 obtain ⟨l₁, l₂, h₈⟩:= h₈
 subst l
-have ⟨h₈, h₉⟩ := path_decomposition g x z y l₁ l₂ h₆
-have g₁ : z ∈ b' \/ ¬ z ∈ b' := by tauto
-have g₂ : z ∈ b  \/ ¬ z ∈ b  := by tauto
-obtain ⟨h₄, _⟩ := h₄
-obtain ⟨_, h₇⟩ := h₅
-cases g₁ <;> cases g₂ <;> constructor <;> try assumption
+have ⟨h₈, h₉⟩ := path_decomposition g x z y l₁ l₂ h₇
+by_cases z ∈ b' <;> by_cases z ∈ b <;> constructor <;> try assumption
 . intros g₃
-  apply no_black_to_white_no_path g b h₁ l₂ z y g₃ h₇ h₉
+  apply no_black_to_white_no_path g b h₁ l₂ z y g₃ (by assumption) h₉
 . exfalso
   apply no_black_to_white_no_path g b' h₂ l₁ x z h₄ <;> assumption
 . intros _
@@ -216,7 +223,8 @@ cases g₁ <;> cases g₂ <;> constructor <;> try assumption
   apply no_black_to_white_no_path g b' h₂ l₁ x z h₄ <;> assumption
 
 
-theorem wff_stack_white_extension [DirectedGraph V Graph]
+theorem wff_stack_white_extension {V Graph: Type*}
+                                  [DirectedGraph V Graph]
                                   [BEq V] [LawfulBEq V]
                                   (g : Graph) :
 ∀ grey grey' (s s': List V),
@@ -225,13 +233,12 @@ theorem wff_stack_white_extension [DirectedGraph V Graph]
   grey ⊆ grey' ->
   ∀ x, x ∈ s' -> x ∈ s \/ x ∈ grey -> False := by
 simp [wff_stack_G1, reachable_before_same_scc, wff_color]
-intros grey _ s s' _ _ _ _ _ _ h₅ _ g₂ _ _ _ _ g₁ x _ g₄
-cases g₄ with
-| inl g₄ => specialize g₂ x
-            rw [num_occ_concat] at g₂
-            rw [mem_num_occ] at *
-            simp_all
-            omega
-| inr g₄ => apply h₅ x
-            . simp_all
-            . apply g₁ g₄
+intros grey _ s s' _ _ _ _ _ _ h₅ _ g₂ _ _ _ _ g₁ x g₄
+constructor <;> intros h <;> simp_all
+. unfold List.Nodup at g₂
+  rw [List.pairwise_append] at g₂
+  obtain ⟨_, _, g₂⟩ := g₂
+  apply g₂ x (by assumption) x (by assumption) rfl
+. apply h₅ x
+  . simp_all
+  . apply g₁ h
