kosaraju-tarjan-lean4/Kosaraju.lean
@@ -1,5 +1,20 @@
 -- This module serves as the root of the `Kosaraju` library.
 -- Import modules here that should be built as part of the library.
-import «Graph».AdjacencyTable
-import «Kosaraju».Basic
-import «Tarjan».Basic
+import ListHelper.Simplelist
+import ListHelper.Rip
+import ListHelper.Union
+import ListHelper.Rank
+
+import Graph.DirectedGraph
+import Graph.AdjacencyTable
+import Graph.Scc
+import Graph.ReachableBefore
+
+import Kosaraju.Dfs2
+import Kosaraju.Dfs1
+import Kosaraju.Grail
+import Kosaraju.Basic
+
+import Tarjan.Env
+import Tarjan.Dfs
+import Tarjan.Basic
