kosaraju-tarjan-lean4/Kosaraju/Dfs2.lean
@@ -3,18 +3,20 @@ import Graph.Scc
 import Graph.ReachableBefore
 import ListHelper.Rank
 import Mathlib.Tactic.Tauto
-import Std.Data.List.Lemmas
+import Init.Data.List.Lemmas
 
-structure Funnel [DirectedGraph V Graph] [BEq V] [LawfulBEq V]
-                  (graph: Graph)
-                  (roots black_stack grays : List V)
+structure Funnel {V Graph: Type*}
+                 [DirectedGraph V Graph] [BEq V] [LawfulBEq V]
+                 (graph: Graph)
+                 (roots black_stack grays : List V)
 where
   stack : List V
   p₁ : wff_color graph stack grays
   p₂ : roots ⊆ stack ++ grays
   monotony: ∃ s', stack = s' ++ black_stack /\ access_from_set graph roots s'
 
-def dfs2 [DirectedGraph V Graph] [BEq V] [LawfulBEq V]
+def dfs2 {V Graph: Type*}
+         [instance_graph : DirectedGraph V Graph] [BEq V] [LawfulBEq V]
          (graph: Graph)
          (roots black_stack grays : List V)
          (h₁: roots ⊆ DirectedGraph.vertices graph)
@@ -23,7 +25,7 @@ def dfs2 [DirectedGraph V Graph] [BEq V] [LawfulBEq V]
          : Funnel graph roots black_stack grays := match roots with
 | List.nil => {
   stack := black_stack
-  p₁ := by assumption
+  p₁ := h₃
   p₂ := by tauto
   monotony := by use []; tauto
 }
@@ -56,23 +58,18 @@ def dfs2 [DirectedGraph V Graph] [BEq V] [LawfulBEq V]
   else
     let h₄ := by simp_all
     have h₅ := by simp [wff_color] at *
-                  constructor
+                  repeat any_goals apply And.intro
+                  any_goals tauto
                   . simp_all
-                    . intros y h₁ h₂
-                      subst y
-                      apply h₅
-                      tauto
-                  . constructor
-                    . simp [no_black_to_white]
-                      intros a b
-                      obtain ⟨_, h₃, _, _⟩ := h₃
-                      specialize h₃ a b
-                      tauto
-                    . rw [simplelist_tl]
-                      simp_all
-                      tauto
-    let v : List V := (DirectedGraph.vertices graph)
-    let termination_proof: grays.length < v.length := by
+                    intros y h₁ h₂
+                    subst y
+                    tauto
+                  . simp [no_black_to_white]
+                    intros a b
+                    obtain ⟨_, h₃, _, _⟩ := h₃
+                    specialize h₃ a b
+                    tauto
+    have : grays.length < (instance_graph.vertices graph).length := by
       apply simplelist_size_2
       . tauto
       . simp [wff_color] at h₃
@@ -83,7 +80,6 @@ def dfs2 [DirectedGraph V Graph] [BEq V] [LawfulBEq V]
         . rename_i h
           simp [*] at h
           intro g
-          apply h
           tauto
     let ⟨stack, p₃, p₄, monotony⟩ := dfs2 graph (DirectedGraph.succ graph x) black_stack (List.cons x grays) (by apply succ_valid; tauto) h₄ h₅
     have h₇ : ¬ x ∈ stack := by
@@ -113,37 +109,30 @@ def dfs2 [DirectedGraph V Graph] [BEq V] [LawfulBEq V]
       . obtain ⟨s', _, _⟩ := monotony
         subst stack
         simp [wff_color, reachable_before_same_scc] at p₃
-        obtain ⟨p₃, _⟩ := p₃
-        apply p₃ b
-        . have h : x :: s' ++ black_stack = s1 ++ black_stack := by tauto
-          have h := List.append_inj_left' h rfl
-          subst s1
-          cases h₆ <;> try tauto
-          rename_i g _ _ _ _ __ _ h₆
-          simp at g
-          exfalso
-          apply g
-          tauto
-        . tauto
-      . have h₆: simplelist (List.cons x stack) := by
-          rw [simplelist_tl]
+        casesm* _ ∧ _
+        have h : x :: s' ++ black_stack = s1 ++ black_stack := by tauto
+        have h := List.append_inj_left' h rfl
+        subst s1
+        cases h₆ <;> try tauto
+        rename_i g _ _ _ _ _ _
+        specialize g b (by tauto)
+        tauto
+      . have h₆: List.Nodup (List.cons x stack) := by
+          rw [List.nodup_cons]
           constructor <;> try assumption
           simp [wff_color, reachable_before_same_scc] at *
           tauto
-        specialize h₆ b
-        rw [h, num_occ_concat] at h₆
-        rw [mem_num_occ] at *
-        omega
+        unfold List.Nodup at h₆
+        rw [h] at h₆
+        rw [List.pairwise_append] at h₆
+        obtain ⟨_, _, h₆⟩ := h₆
+        apply h₆ b (by assumption) b (by assumption) rfl
     have g₉: no_path_out_of_in graph black_stack (List.cons x stack) := by
       apply no_edge_out_of_no_path_out_of_in ; assumption
     have h₆ := by
        simp [wff_color, reachable_before_same_scc] at p₃
        simp [wff_color, reachable_before_same_scc]
-       obtain ⟨p₅, _, ⟨p₇, p₉⟩⟩ := p₃
-       rw [simplelist_tl] at *
        simp_all
-       intros a h₃ h₄
-       apply p₅ <;> tauto
     let ⟨stack, p₃, p₄, monotony⟩ := dfs2 graph roots (List.cons x stack) grays (by tauto) (by tauto) h₆
     {
       stack := stack
