kosaraju-tarjan-lean4/ListHelper/Simplelist.lean
@@ -1,99 +1,20 @@
-import Std.Data.List.Basic
-import Std.Data.List.Lemmas
+import Init.Data.List.Basic
+import Init.Data.List.Lemmas
+import Init.Data.List.Pairwise
 import Mathlib.Tactic.Tauto
 
-def num_occ [BEq α] [LawfulBEq α] (x : α) (s : List α) : Nat :=
-match s with
-| List.nil => 0
-| List.cons y s => if x == y then
-                    Nat.succ (num_occ x s)
-                  else
-                    num_occ x s
-
-@[simp] theorem num_occ_concat [BEq α] [LawfulBEq α] :
- ∀ (x : α) l₁ l₂, num_occ x (l₁ ++ l₂) = num_occ x l₁ + num_occ x l₂ := by
-intro x l₁
-induction l₁ <;> simp [num_occ] ; split <;> simp_all
-omega
-
-theorem mem_num_occ [BEq α] [LawfulBEq α] :
- ∀ (x : α) l, x ∈ l ↔ num_occ x l > 0 := by
-intros x l
-induction l <;> simp [num_occ] ; split <;> simp_all
-
-theorem mem_num_occ_0 [BEq α] [LawfulBEq α] :
- ∀ (x : α) l, ¬ x ∈ l ↔ num_occ x l = 0 := by
-intros x l
-induction l <;> simp [num_occ] ; split <;> simp_all
-
-def simplelist [BEq α] [LawfulBEq α] (s : List α) : Prop :=
-∀ x, num_occ x s <= 1
-
-theorem simplelist_tl [BEq α] [LawfulBEq α] :
- ∀ (x : α) l, simplelist (List.cons x l) ↔ simplelist l /\ ¬ x ∈ l
-:= by
-simp [simplelist, num_occ]
-intros x s1
-constructor
-. intros h₁
-  constructor
-  . intros y
-    specialize h₁ y
-    split at h₁ <;> omega
-  . specialize h₁ x
-    split at h₁
-    . revert h₁
-      induction s1
-      . simp_all
-      . simp [num_occ]
-        split <;> simp_all
-        omega
-    . simp_all
-. intros h₁ y
-  split <;> simp_all
-  subst y
-  obtain ⟨_, h₁⟩ := h₁
-  rw [mem_num_occ_0] at h₁
-  omega
-
-theorem simplelist_size [BEq α] [LawfulBEq α] :
-∀ (l₁ l₂: List α), l₁ ⊆ l₂ -> simplelist l₁ -> l₁.length ≤ l₂.length := by
-intros l₁
-induction l₁
-. simp_all
-. intros l₂ h₁ h₂
-  rename_i a l₁ induction_step
-  rw [simplelist_tl] at h₂
-  simp_all
-  obtain ⟨h₁, h₃⟩ := h₁
-  have h₄: ∃ l₃ l₄, l₂ = l₃ ++ List.cons a l₄ := by apply List.append_of_mem; assumption
-  obtain ⟨l₃, l₄, h₄⟩ := h₄
-  subst l₂
-  specialize induction_step (l₃ ++ l₄)
-  have : l₁ ⊆ l₃ ++ l₄ := by
-    simp [Subset, List.Subset]
-    intros x h₆
-    specialize h₃ h₆
-    simp_all
-    cases h₃ with
-    | inl _ => tauto
-    | inr h₃ => cases h₃
-                . subst x
-                  tauto
-                . tauto
-  simp_all
-  omega
+variable {α : Type*}
 
 theorem simplelist_size_2 [BEq α] [LawfulBEq α] :
-∀ (l₁ l₂: List α), l₁ ⊆ l₂ -> simplelist l₁ -> (∃ b, b ∈ l₂ /\ ¬ b ∈ l₁) -> l₁.length < l₂.length := by
+∀ (l₁ l₂: List α), l₁ ⊆ l₂ -> List.Nodup l₁ -> (∃ b, b ∈ l₂ /\ ¬ b ∈ l₁) -> l₁.length < l₂.length := by
 intros l₁
 induction l₁
 . simp_all
-  intros l₂ _ x h
+  intros l₂ _ x
   rw [List.length_pos]
   intro
   subst l₂
-  cases h
+  tauto
 . intros l₂ h₁ h₂ h₃
   simp_all
   obtain ⟨h₁, h₄⟩ := h₁
@@ -101,7 +22,6 @@ induction l₁
   have h₅: ∃ l₃ l₄, l₂ = l₃ ++ List.cons c l₄ := by apply List.append_of_mem; assumption
   obtain ⟨l₃, l₄, h₅⟩ := h₅
   subst l₂
-  rw [simplelist_tl] at h₂
   have : l₁ ⊆ l₃ ++ l₄ := by
     simp [Subset, List.Subset]
     intros x h₆
@@ -118,28 +38,14 @@ induction l₁
   simp_all
   have : b ∈ l₃ \/ b ∈ l₄ := by cases h₃ <;> tauto
   specialize induction_step b
-  have : ¬ b ∈ l₁ := by intro h; apply h₉; tauto
+  have : ¬ b ∈ l₁ := by intro h; tauto
   simp_all
   omega
-
-theorem simplelist_l [BEq α] [LawfulBEq α] {l₁ l₂ : List α}:
-simplelist (l₁ ++ l₂) -> simplelist l₁ := by
-intros h x
-specialize h x
-simp at h
-omega
-
-theorem simplelist_r [BEq α] [LawfulBEq α] {l₁ l₂ : List α}:
-simplelist (l₁ ++ l₂) -> simplelist l₂ := by
-intros h x
-specialize h x
-simp at h
-omega
 
 theorem simplelist_uniq [BEq α] [LawfulBEq α] {x : α} :
 ∀ l₁ l₃ l₂ l₄: List α,
 l₁ ++ x :: l₂ = l₃ ++ x :: l₄ ->
-simplelist (l₁ ++ x :: l₂ ) ->
+List.Nodup (l₁ ++ x :: l₂) ->
 l₁ = l₃ /\ l₂ = l₄ := by
 intro l₁
 induction l₁
@@ -150,21 +56,19 @@ all_goals intros l₂ l₄ h h₁ h₃
 any_goals subst x
 any_goals subst l₂
 all_goals rename_i y _ _
-. specialize h₃ y
-  simp [num_occ] at h₃
-  omega
+. intros _
+  apply h₃
+  simp
 . match l₂ with
   | [] => simp at h₁
           obtain ⟨h₁, _⟩ := h₁
           subst y
-          specialize h₃ x
-          simp [num_occ] at h₃
-          omega
-  | z :: l₂ => simp at h₁
-               obtain ⟨h₁, h₅⟩ := h₁
-               subst z
-               rename_i l₁ induction_step _
-               rw [simplelist_tl] at h₃
-               obtain ⟨h₃, _⟩ := h₃
-               specialize induction_step _ _ _ h₅ h₃
-               tauto
+          intros _
+          tauto
+  | z :: l₂ =>  simp at h₁
+                obtain ⟨h₁, h₅⟩ := h₁
+                subst z
+                rename_i l₁ induction_step _
+                intros _ _ h₆
+                specialize induction_step _ _ _ h₅ h₆
+                simp_all
