kosaraju-tarjan-lean4/README.md
@@ -1,3 +1,5 @@
+# Kosaraju
+
 ```
 lake build
 ```
